Update examples.

examples/Calculemus2011.v
@@ -1,36 +1,132 @@
 Require Import ARDyadics CRArith ARexp ARpi ARarctan.
 Require Import CRArith Compress CRexp CRpi CRarctan.
 
-Definition answer (n:positive) (r : CR) : Z :=
- let m := (iter_pos n _ (Pmult 10) 1%positive) in
- let (a,b) := (approximate r (1#m)%Qpos)*m in
- Zdiv a b.
+Definition eval (n:positive) (r : CR) : Q :=
+ let m := iter_pos n _ (Pmult 10) 1%positive in approximate r (1#m)%Qpos.
 
-Let ARtest1 : CR := ARtoCR (ARpi : fastAR).
+Definition deval (n:positive) (r : fastAR) : fastD :=
+ let m := iter_pos n _ (Pmult 10) 1%positive in approximate r (1#m)%Qpos.
+
+Let ARtest1 : fastAR := ARpi.
 Let CRtest1 : CR := CRpi.
 
-Let ARtest2 : CR := ARtoCR (ARexp (ARcompress (ARexp (ARcompress (AQexp (1 ≪ (-1) : fastD)))))).
+Let ARtest2 : fastAR := ARexp (ARcompress (ARexp (ARcompress (AQexp (1 ≪ (-1)))))).
 Let CRtest2 : CR := exp (compress (exp (compress (rational_exp (1#2))))).
 
-Let ARtest3 : CR := ARtoCR (ARexp (ARcompress ARpi) - ARpi : fastAR).
+Let ARtest3 : fastAR := ARexp (ARcompress ARpi) - ARpi.
 Let CRtest3 : CR := exp (compress CRpi) - CRpi.
 
-Let ARtest4 : CR := ARtoCR (ARarctan (ARcompress (ARpi : fastAR))).
+Let ARtest4 : fastAR := ARarctan (ARcompress ARpi).
 Let CRtest4 : CR := arctan (compress CRpi).
 
-Time Eval vm_compute in (answer 300 ARtest1).
-Time Eval vm_compute in (answer 300 CRtest1).
-Time Eval vm_compute in (answer 1750 ARtest1).
+Time Eval vm_compute in (deval 300 ARtest1).
+Time Eval vm_compute in (eval 300 CRtest1).
+Time Eval vm_compute in (deval 2000 ARtest1).
 
-Time Eval vm_compute in (answer 25 ARtest2).
-Time Eval vm_compute in (answer 25 CRtest2).
-Time Eval vm_compute in (answer 450 ARtest2).
+Time Eval vm_compute in (deval 25 ARtest2).
+Time Eval vm_compute in (eval 25 CRtest2).
+Time Eval vm_compute in (deval 450 ARtest2).
 
-Time Eval vm_compute in (answer 25 ARtest3).
-Time Eval vm_compute in (answer 25 CRtest3).
-Time Eval vm_compute in (answer 425 ARtest3).
+Time Eval vm_compute in (deval 25 ARtest3).
+Time Eval vm_compute in (eval 25 CRtest3).
+Time Eval vm_compute in (deval 425 ARtest3).
 
-Time Eval vm_compute in (answer 25 ARtest4).
-Time Eval vm_compute in (answer 25 CRtest4).
-Time Eval vm_compute in (answer 85 ARtest4).
+Time Eval vm_compute in (deval 25 ARtest4).
+Time Eval vm_compute in (eval 25 CRtest4).
+Time Eval vm_compute in (deval 85 ARtest4).
 
+(* Finally, we compare our sqrt with an implementation not using type classes *)
+Require Import ARroot dyadics.
+
+Let n := Eval compute in (10 * 10 * 10 * 10)%nat.
+Let ARroot_test : nat -> fastD * fastD := AQsqrt_loop (a:=2).
+
+Time Eval vm_compute in (
+  (fun _ _ _ _ _ _ _ _ _ _ => true)
+  (snd (ARroot_test n))
+  (snd (ARroot_test n))
+  (snd (ARroot_test n))
+  (snd (ARroot_test n))
+  (snd (ARroot_test n))
+  (snd (ARroot_test n))
+  (snd (ARroot_test n))
+  (snd (ARroot_test n))
+  (snd (ARroot_test n))
+  (snd (ARroot_test n))).
+
+Require Import BigZ.
+Open Scope bigZ_scope.
+
+Notation bigD := (Dyadic bigZ).
+
+Definition BigD_0 : bigD := (0 $ 0).
+Definition BigD_1 : bigD := (1 $ 0).
+Definition BigD_2 : bigD := (2 $ 0).
+Definition BigD_4 : bigD := (4 $ 0).
+
+Definition BigD_plus (x y : bigD) : bigD := 
+  match BigZ.compare (expo x) (expo y) with
+  | Gt => BigZ.shiftl (mant x) (expo x - expo y) + mant y $ BigZ.min (expo x) (expo y)
+  | _ => mant x + BigZ.shiftl (mant y) (expo y - expo x) $ BigZ.min (expo x) (expo y)
+  end.
+
+Definition BigD_opp (x : bigD) : bigD := -mant x $ expo x.
+
+Definition BigD_mult (x y : bigD) : bigD := mant x * mant y $ expo x + expo y.
+
+Definition BigD_shiftl (x : bigD) (n : bigZ) : bigD := mant x $ expo x + n.
+
+Definition BigD_compare (x y : bigD) : comparison := 
+  match BigZ.compare (expo x) (expo y) with
+  | Gt => BigZ.compare (BigZ.shiftl (mant x) (expo x - expo y)) (mant y)
+  | _ => BigZ.compare (mant x) (BigZ.shiftl (mant y) (expo y - expo x))
+  end.
+
+Fixpoint root_loop_alt (x : bigD) (n : nat) : bigD * bigD :=
+  match n with
+  | O => (x, BigD_0)
+  | S n => let (r, s) := root_loop_alt x n in
+     match BigD_compare (BigD_plus s BigD_1) r with
+     | Gt => (BigD_shiftl r 2, BigD_shiftl s 1)
+     | _ => (BigD_shiftl (BigD_plus r (BigD_opp (BigD_plus s BigD_1))) 2, BigD_shiftl (BigD_plus s BigD_2) 1)
+     end
+  end.
+
+Time Eval vm_compute in (
+  (fun _ _ _ _ _ _ _ _ _ _ => true)
+  (snd (root_loop_alt BigD_2 n))
+  (snd (root_loop_alt BigD_2 n))
+  (snd (root_loop_alt BigD_2 n))
+  (snd (root_loop_alt BigD_2 n))
+  (snd (root_loop_alt BigD_2 n))
+  (snd (root_loop_alt BigD_2 n))
+  (snd (root_loop_alt BigD_2 n))
+  (snd (root_loop_alt BigD_2 n))
+  (snd (root_loop_alt BigD_2 n))
+  (snd (root_loop_alt BigD_2 n))).
+
+(* As suggested by Laurent Théry, mult is more efficient than shiftl in case the size of bigN is 
+    large enough. By increasing size in theories/Numbers/Natural/BigN/NMake_gen.ml to 12 
+    the following is faster. *)
+Fixpoint root_loop_alt_mult (x : bigD) (n : nat) : bigD * bigD :=
+  match n with
+  | O => (x, BigD_0)
+  | S n => let (r, s) := root_loop_alt_mult x n in
+     match BigD_compare (BigD_plus s BigD_1) r with
+     | Gt => (BigD_mult BigD_4 r, BigD_mult BigD_2 s)
+     | _ => (BigD_mult BigD_4 (BigD_plus r (BigD_opp (BigD_plus s BigD_1))), BigD_mult BigD_2 (BigD_plus s BigD_2))
+     end
+  end.
+
+Time Eval vm_compute in (
+  (fun _ _ _ _ _ _ _ _ _ _ => true)
+  (snd (root_loop_alt_mult BigD_2 n))
+  (snd (root_loop_alt_mult BigD_2 n))
+  (snd (root_loop_alt_mult BigD_2 n))
+  (snd (root_loop_alt_mult BigD_2 n))
+  (snd (root_loop_alt_mult BigD_2 n))
+  (snd (root_loop_alt_mult BigD_2 n))
+  (snd (root_loop_alt_mult BigD_2 n))
+  (snd (root_loop_alt_mult BigD_2 n))
+  (snd (root_loop_alt_mult BigD_2 n))
+  (snd (root_loop_alt_mult BigD_2 n))).
