examples/RealDyadic.v
@@ -1,68 +1,30 @@
-Require Import ARDyadics CRArith ARexp ARpi ARarctan.
+Require Import BigZ ARDyadics CRArith ARexp ARpi ARarctan ARroot.
 
-Definition answer (n:positive) (r : CR) : Z :=
- let m := (iter_pos n _ (Pmult 10) 1%positive) in
- let (a,b) := (approximate r (1#m)%Qpos)*m in
- Zdiv a b.
-(*
-Let ARtest : CR := ARtoCR (2 * ARexp (ARexp (AQexp (1 : fastD)))).
-Time Eval vm_compute in (answer 200 ARtest).
+Definition answer (n:positive) (r : fastAR) : bigZ :=
+ let m := (iter_pos n _ (Pmult 10) 1%positive) in 
+ let (a, b) := (approximate r (1#m)%Qpos : fastD) * 'Zpos m in 
+ BigZ.shiftl a b.
 
-Let ARtest2 : CR := ARtoCR ('(ZtofastD 4) + AQexp (ZtofastD 10)).
-Time Eval vm_compute in (answer 1500 ARtest2).
+Let ARtest : fastAR := 2 * ARexp (ARexp (AQexp 1)).
+Time Eval vm_compute in (answer 150 ARtest).
 
-Let ARtest3 : CR := ARtoCR (ARpi : fastAR).
-Time Eval vm_compute in (answer 1500 ARtest3).
+Let ARtest2 : fastAR := '(4 : Z) + AQexp ('(10 : Z)).
+Time Eval vm_compute in (answer 1250 ARtest2).
 
-Let ARtest4 : CR := ARtoCR (ARexp ARpi - ARpi : fastAR).
-Time Eval vm_compute in (answer 350 ARtest4).
-*)
+Let ARtest3 : fastAR := ARpi.
+Time Eval vm_compute in (answer 750 ARtest3).
 
-Timeout 3 Let ARtest5 : CR := ARtoCR (ARarctan (ARcompress (ARpi : fastAR))).
-(* (ARcompress (AQexp (1 : fastD)))). *)
-Timeout 10 Time Eval vm_compute in (answer 10 ARtest5).
+Let ARtest4 : fastAR := ARexp ARpi - ARpi.
+Time Eval vm_compute in (answer 200 ARtest4).
 
-(*
+Let ARtest5 : fastAR := ARarctan (ARcompress ARpi).
+Time Eval vm_compute in (answer 35 ARtest5).
 
-Definition half : fastD := 1 $ (-1)%bigZ.
-(*
-Lemma yada2 : -(1) ≤ ('half : Q) ≤ 0.
-Proof.
-Admitted.
+Let ARtest6 : fastAR := ARsqrt 2.
+Time Eval vm_compute in (answer 1000 ARtest6).
 
-Let test := ARAlternatingSum.ARInfAltSum_length (ARexpSequence half)
-   (zl:=CRexp.expSequence_zl (CRexp.Qle_ZO_flip yada2)).
+Let ARtest7 : fastAR := ARsqrt (ARexp 1).
+Time Eval vm_compute in (answer 500 ARtest7).
 
-Time Eval vm_compute in (test (-100)).
-
-Time Eval vm_compute in (ARAlternatingSum.ARAltSum (CRseries.powers (-half)) (CRseries.factorials) 8 (-200)).
-*)
-Definition answer (n:positive) (r : CR) : Z :=
- let m := (iter_pos n _ (Pmult 10) 1%positive) in
- let (a,b) := (approximate r (1#m)%Qpos)*m in
- Zdiv a b.
-
-Timeout 3 Let ARtest : CR := ARtoCR (ARexp (ARexp (AQexp (1 : fastD)))).
-Timeout 3 Let ARtest2 : CR := ARtoCR (AQexp ('(10 : Z) : fastD)).
-
-Let n : positive := 2000%positive.
-
-Timeout 30 Time Eval vm_compute in (answer n ARtest2).
-
-(*
-Let CRtest : CR := CRexp.exp (Compress.compress (CRexp.exp (Compress.compress (CRexp.rational_exp (1#2))))).
-Timeout 10 Time Eval vm_compute in (answer n CRtest).
-
-Let ARtest2 : CR := ARtoCR (AQexp (1 $ 2 : fastD)).
-
-Let boundQ (a : Q) := (3#1)^(Zdiv (Qnum (- a)) (Qden (- a))).
-
-Timeout 10 Eval vm_compute in (boundQ 1).
-Timeout 10 Eval vm_compute in (proj1_sig (AQexp_inv_pos_bound (1 : fastD))).
-Let CRtest : CR := CRexp.rational_exp (4).
-
-Let n : positive := 1000%positive.
-Timeout 10 Time Eval vm_compute in (answer n ARtest2).
-Time Eval vm_compute in (answer n CRtest).
-*)
-*)
+Let ARtest8 : fastAR := ARexp (ARsqrt 2).
+Time Eval vm_compute in (answer 200 ARtest8).
